定義に不備があったので修正、stepとの同地関係を証明

practice/TaPL/coq/arith/ocaml/eval.ml
@@ -19,80 +19,51 @@ let rec isnumericval = function
 | Succ t1 -> isnumericval t1
 | _ -> False
 
+(** val isval : term -> bool **)
+
+let rec isval t = match t with
+| Tru -> True
+| Fls -> True
+| _ -> isnumericval t
+
 type optiont =
 | Some of term
-| Value of term
 | None
 
 (** val eval1 : term -> optiont **)
 
-let rec eval1 t = match t with
+let rec eval1 = function
 | If (t1, t2, t3) ->
-  (match t1 with
-   | Tru -> Some t2
-   | Fls -> Some t3
-   | _ -> (match eval1 t1 with
-           | Some t1' -> Some (If (t1', t2, t3))
-           | _ -> None))
+  (match isval t1 with
+   | True -> (match t1 with
+              | Tru -> Some t2
+              | Fls -> Some t3
+              | _ -> None)
+   | False -> (match eval1 t1 with
+               | Some t1' -> Some (If (t1', t2, t3))
+               | None -> None))
 | Succ t1 ->
   (match isnumericval t1 with
-   | True -> Value t
+   | True -> None
    | False -> (match eval1 t1 with
                | Some t1' -> Some (Succ t1')
-               | _ -> None))
+               | None -> None))
 | Pred t1 ->
-  (match t1 with
-   | O -> Some O
-   | Succ t1' ->
-     (match isnumericval t1' with
-      | True -> Some t1'
-      | False -> (match eval1 t1' with
-                  | Some t1'' -> Some (Pred (Succ t1''))
-                  | _ -> None))
-   | _ -> (match eval1 t1 with
-           | Some t1' -> Some (Pred t1')
-           | _ -> None))
-| Iszero t1 ->
-  (match t1 with
-   | O -> Some Tru
-   | Succ t1' ->
-     (match isnumericval t1' with
-      | True -> Some t1'
-      | False -> (match eval1 t1' with
-                  | Some t1'' -> Some (Pred (Succ t1''))
-                  | _ -> None))
-   | _ -> (match eval1 t1 with
-           | Some t1' -> Some (Pred t1')
-           | _ -> None))
-| _ -> Value t
-
-(** val bstep : term -> optiont **)
-
-let rec bstep t = match t with
-| If (t1, t2, t3) ->
-  (match bstep t1 with
-   | Value t0 -> (match t0 with
-                  | Tru -> bstep t2
-                  | Fls -> bstep t3
-                  | _ -> None)
-   | _ -> None)
-| Succ t1 -> (match bstep t1 with
-              | Value t0 -> (match t0 with
-                             | O -> Value (Succ t1)
-                             | _ -> None)
+  (match isnumericval t1 with
+   | True -> (match t1 with
+              | O -> Some O
+              | Succ nv1 -> Some nv1
               | _ -> None)
-| Pred t1 ->
-  (match bstep t1 with
-   | Value t0 -> (match t0 with
-                  | O -> Value O
-                  | Succ t1' -> Value t1'
-                  | _ -> None)
-   | _ -> None)
+   | False -> (match eval1 t1 with
+               | Some t1' -> Some (Pred t1')
+               | None -> None))
 | Iszero t1 ->
-  (match bstep t1 with
-   | Value t0 -> (match t0 with
-                  | O -> Value Tru
-                  | Succ _ -> Value Fls
-                  | _ -> None)
-   | _ -> None)
-| _ -> Value t
+  (match isnumericval t1 with
+   | True -> (match t1 with
+              | O -> Some Tru
+              | Succ _ -> Some Fls
+              | _ -> None)
+   | False -> (match eval1 t1 with
+               | Some t1' -> Some (Iszero t1')
+               | None -> None))
+| _ -> None
