practice/TaPL/coq/arith/chap4.v
@@ -27,58 +27,51 @@ Fixpoint isval (t: term) : bool :=
 
 Inductive optiont : Type :=
 | Some (t: term)
-| value (t: term)
 | None.
 
 Fixpoint eval1 (t: term) : optiont :=
   match t with
   | If t1 t2 t3 =>
-    match t1 with
-    | tru => Some t2
-    | fls => Some t3
-    | _ => match (eval1 t1) with
-           | Some t1' => Some (If t1' t2 t3)
-           | _ => None
-           end
-    end
+    if (isval t1) then
+      match t1 with
+      | tru => Some t2
+      | fls => Some t3
+      | _ => None
+      end else
+      match (eval1 t1) with
+      | Some t1' => Some (If t1' t2 t3)
+      | _ => None
+      end
   | succ t1 =>
     if isnumericval t1 then
-      value t else
+      None else
       match (eval1 t1) with
       | Some t1' => Some (succ t1')
       | _ => None
       end
   | pred t1 =>
-    match t1 with
-    | O => Some O
-    | succ t1' =>
-      if isnumericval t1' then
-        Some t1' else
-        match (eval1 t1') with
-        | Some t1'' => Some (pred (succ t1''))
-        | _ => None
-        end
-    | _ => match (eval1 t1) with
-           | Some t1' => Some (pred t1')
-           | _ => None
-           end
-    end
+    if (isnumericval t1) then
+      match t1 with
+      | O => Some O
+      | succ nv1 => Some nv1
+      | _ => None
+      end else
+      match (eval1 t1) with
+      | Some t1' => Some (pred t1')
+      | _ => None
+      end
   | iszero t1 =>
-    match t1 with
-    | O => Some tru
-    | succ t1' =>
-      if isnumericval t1' then
-        Some t1' else
-        match (eval1 t1') with
-        | Some t1'' => Some (pred (succ t1''))
-        | _ => None
-        end
-    | _ => match (eval1 t1) with
-           | Some t1' => Some (pred t1')
-           | _ => None
-           end
-    end
-  | _ => value t
+    if (isnumericval t1) then
+      match t1 with
+      | O => Some tru
+      | succ _ => Some fls
+      | _ => None
+      end else
+      match (eval1 t1) with
+      | Some t1' => Some (iszero t1')
+      | _ => None
+      end
+  | _ => None
   end.
 
 
@@ -94,68 +87,214 @@ Ltac solve_by_invert :=
   solve_by_inverts 1.
 
 Theorem eval1value : forall t1,
-    eval1 t1 = value t1 <-> isval t1 = true.
+    isval t1 = true -> eval1 t1 = None.
+Proof.
+  intros. induction t1; try solve_by_inverts 2; try reflexivity.
+  inversion H. simpl. rewrite H1; auto.
+Qed.
+
+
+Extraction "ocaml/eval.ml" eval1.
+
+Inductive NatValue: term -> Prop :=
+| nv_O : NatValue O
+| nv_S : forall nv1, NatValue nv1 -> NatValue (succ nv1).
+
+Inductive Pvalue: term -> Prop :=
+| v_tru : Pvalue tru
+| v_fls : Pvalue fls
+| v_nat : forall t1, NatValue t1 -> Pvalue t1.
+
+Reserved Notation " t '-->' t' " (at level 40).
+Inductive step: term -> term -> Prop :=
+| E_IfTrue : forall t2 t3,
+    If tru t2 t3 --> t2
+| E_IfFalse : forall t2 t3,
+    If fls t2 t3 --> t3
+| E_If : forall t1 t1' t2 t3,
+    t1 --> t1' ->
+    If t1 t2 t3 --> If t1' t2 t3
+| E_Succ : forall t1 t1',
+    t1 --> t1' -> succ t1 --> succ t1'
+| E_PredZero :
+    pred O --> O
+| E_PredSucc : forall nv1,
+    NatValue nv1 -> pred (succ nv1) --> nv1
+| E_Pred : forall t1 t1',
+    t1 --> t1' -> pred t1 --> pred t1'
+| E_IsZeroZero :
+    iszero O --> tru
+| E_IsZeroSucc : forall nv1,
+    NatValue nv1 -> iszero (succ nv1) --> fls
+| E_IsZero : forall t1 t1',
+    t1 --> t1' -> iszero t1 --> iszero t1'
+
+  where " t '-->' t' " := (step t t').
+
+
+Lemma nat_value : forall t,
+    NatValue t <-> isnumericval t = true.
 Proof.
   split; intros.
   -
-    induction t1; try reflexivity.
-    + inversion H.
-      destruct t1_1; try solve_by_invert.
-      induction (eval1 (If t1_1_1 t1_1_2 t1_1_3)); try solve_by_invert.
-      destruct (eval1 (succ t1_1)); try solve_by_invert.
-      destruct (eval1 (pred t1_1)); try solve_by_invert.
-      destruct (eval1 (iszero t1_1)); try solve_by_invert.
-    + inversion H.
-      simpl.
-      destruct (isnumericval t1)eqn:IH; auto.
-      destruct (eval1 t1); inversion H1.
-    + inversion H.
-      destruct t1; try solve_by_invert.
-      destruct (eval1 (If t1_1 t1_2 t1_3)); try solve_by_invert.
-      destruct (isnumericval t1). inversion H1.
-      destruct (eval1  t1); inversion H1.
-      destruct (eval1 (pred t1)); inversion H1.
-      destruct (eval1 (iszero t1)); inversion H1.
-    + inversion H.
-      destruct t1; try solve_by_invert.
-      destruct (eval1 (If t1_1 t1_2 t1_3)); try solve_by_invert.
-      destruct (isnumericval t1). inversion H1.
-      destruct (eval1  t1); inversion H1.
-      destruct (eval1 (pred t1)); inversion H1.
-      destruct (eval1 (iszero t1)); inversion H1.
+    induction H; auto.
   -
-    induction t1; try reflexivity; try solve_by_invert.
-    + simpl. inversion H. rewrite H1. reflexivity.
+    induction t; try solve_by_invert.
+    apply nv_O. inversion H. apply IHt in H1. apply nv_S; auto.
 Qed.
 
+Lemma isval_Pvalue : forall t,
+    isval t = true <-> Pvalue t.
+Proof.
+  split; intros.
+  -
+    induction t; try solve_by_invert.
+    apply v_tru. apply v_fls.
+    apply v_nat; apply nv_O.
+    inversion H. apply nat_value in H1. apply v_nat. apply nv_S; auto.
+  -
+    induction H; auto.
+    unfold isval. inversion H; auto.
+    simpl. apply nat_value; auto.
+Qed.
+
+Theorem step_eval1_correct : forall t1 t1',
+    eval1 t1 = Some t1' <-> t1 --> t1'.
+Proof.
+  split.
+  -
+    intros. generalize dependent t1'.
+    induction t1; intros; try solve_by_invert.
+    +
+      inversion H. 
+      induction (isval t1_1).
+      destruct t1_1; try solve_by_invert.
+      inversion H1. apply E_IfTrue.
+      inversion H1. apply E_IfFalse.
+      induction (eval1 t1_1) eqn:IHt1; try solve_by_invert.
+      inversion H1. inversion H1. apply E_If. apply IHt1_1; auto.
+    +
+      inversion H.
+      destruct (isnumericval t1) eqn:IHnum. inversion H1.
+      destruct (eval1 t1) eqn:IH. inversion H1. apply E_Succ. apply IHt1; auto.
+      inversion H1.
+    +
+      inversion H. destruct (isnumericval t1) eqn:IHnum; try solve_by_invert.
+      destruct t1; try solve_by_invert. inversion H1. apply E_PredZero.
+      inversion H1. apply E_PredSucc. inversion IHnum. apply nat_value; subst; auto.
+      destruct (eval1 t1); try solve_by_invert.
+      inversion H1. apply E_Pred. apply IHt1; auto.
+    +
+      inversion H.
+      destruct (isnumericval t1) eqn:IHnum.
+      destruct t1; try solve_by_invert.
+      inversion H1. apply E_IsZeroZero.
+      inversion H1. apply E_IsZeroSucc. inversion IHnum. apply nat_value; auto.
+      destruct (eval1 t1); try solve_by_invert.
+      inversion H1. apply E_IsZero. apply IHt1; auto.
+  -
+    intros. induction H; try reflexivity.
+    +
+      simpl. destruct (isval t1) eqn:IHv.
+      destruct t1; try solve_by_invert. inversion H. inversion IHstep.
+      inversion IHv. rewrite H5 in H4. inversion H4.
+      rewrite IHstep; auto.
+    +
+      simpl. destruct (isnumericval t1) eqn:IHnum.
+      pose proof (eval1value t1).
+      rewrite H0 in IHstep.
+      inversion IHstep.
+      unfold isval. destruct t1; try solve_by_invert; auto.
+
+      destruct (eval1 t1); try solve_by_invert.
+      inversion IHstep; auto.
+    +
+      simpl. apply nat_value in H. rewrite H; auto.
+    +
+      simpl. destruct (isnumericval t1) eqn:IHnum.
+      destruct t1; try solve_by_invert.
+      pose proof (eval1value (succ t1)).
+      rewrite H0 in IHstep. inversion IHstep.
+      simpl. inversion IHnum; auto.
+      destruct (eval1 t1); try solve_by_invert.
+      inversion IHstep; auto.
+    +
+      simpl.
+      destruct (isnumericval nv1) eqn:IHnum; try solve_by_invert; auto.
+      apply nat_value in H. rewrite H in IHnum; inversion IHnum.
+    +
+      simpl.
+      destruct (isnumericval t1) eqn:IHnum.
+      pose proof (eval1value t1). rewrite H0 in IHstep. inversion IHstep.
+      unfold isval. destruct t1; try solve_by_invert; auto.
+      destruct (eval1 t1); try solve_by_invert. inversion IHstep; auto.
+Qed.
+
+
+
+Definition relation (X : Type) := X -> X -> Prop.
+
+Inductive multi {X : Type} (R : relation X) : relation X :=
+  | multi_refl : forall (x : X), multi R x x
+  | multi_step : forall (x y z : X),
+                    R x y ->
+                    multi R y z ->
+                    multi R x z.
+
+Notation multistep := (multi step).
+Notation "t1 '-->*' t2" := (multistep t1 t2) (at level 40).
+
+
+(*停止する保証がないのでbigstepは無理そう*)
+(*
 Fixpoint bstep (t: term) : optiont :=
   match t with
-  | tru => value t
-  | fls => value t
-  | O => value t
+  | tru => Some tru
+  | fls => Some fls
+  | O => Some t
   | If t1 t2 t3 =>
-    match (bstep t1) with
-    | value tru => bstep t2
-    | value fls => bstep t3
-    | _ => None
+    match (eval1 t1) with
+    | Some t1' =>
+      if (isval t1') then
+        match t1' with
+        | tru => bstep t2
+        | fls => bstep t3
+        | _ => None
+        end else bstep (If t1' t2 t3)
+    | None => None
     end
   | succ t1 =>
-    match (bstep t1) with
-    | value O => value (succ t1)
-    | _ => None
+    match (eval1 t1) with
+    | Some t1' =>
+      if (isval t1') then
+        match t1' with
+        | O => Some (succ O)
+        | succ _ => Some (t1')
+        | _ => None
+        end else bstep (succ t1')
+    | None => None
     end
   | pred t1 =>
-    match (bstep t1) with
-    | value (succ t1') => value t1'
-    | value O => value O
+    match (eval1 t1) with
+    | Some t1' =>
+      if (isval t1') then
+        match t1' with
+        | O => Some O
+        | succ nv1 => Some nv1
+        | _ => None
+        end else bstep (pred t1')
     | _ => None
     end
   | iszero t1 =>
-    match (bstep t1) with
-    | value O => value tru
-    | value (succ _) => value fls
+    match (eval1 t1) with
+    | Some t1' =>
+      if (isval t1') then
+        match t1' with
+        | O => Some tru
+        | succ _ => Some fls
+        | _ => None
+        end else bstep (iszero t1')
     | _ => None
     end
   end.
-
-Extraction "ocaml/eval.ml" eval1 bstep.
+*)
